case_study/RiscvPmp/README.md
@@ -10,6 +10,8 @@ Remarks/Comments/Info:
 - keep AccessType simple (i.e. no type parameter for extensions, this is ignored in the PMP related code anyway), but still represent it as a *union* (note that we could opt to represent this as an enum, but this way is more faithful to the (simplified) Sail model)
 - MemoryOpResult is simplified and MemValue can only be a Word (no type param in definition of MemoryOpResult, this complicates EqDec...)
 - Store instructions involve a function mem_write that returns a MemoryOpResult with a boolean value to indicate failure, to keep things simple (point above), I model this as a ty_word where 0 = false and 1 = true
+- the model currently only supports M-mode, so any checks/pattern matches that depend on privileges are simplified to only consider the M-mode case
+- some auxiliary functions that convert bits to enums are dropped, the model uses the enum immediately (example: pmpAddrRange calls a function pmpAddrMatchType_of_bits that converts a bitvector into the corresponding enum value of PmpAddrMatchType)
 
 ## Translation Notes
 Inline function call expressions get translated into
